ironfleet/src/Dafny/Distributed/Concur/Trace.i.dfy
@@ -40,22 +40,4 @@ module TraceModule {
     datatype Entry = Entry(actor:Actor, action:Action)
 
     type Trace = seq<Entry>
-
-    function RestrictTraceToActor(t:Trace, a:Actor) : Trace
-        ensures var t' := RestrictTraceToActor(t, a);
-                forall e {:trigger e in t'} {:trigger e in t, e.actor} :: e in t' <==> e in t && e.actor == a;
-    {
-        if |t| == 0 then
-            []
-        else if t[0].actor == a then
-            [t[0]] + RestrictTraceToActor(t[1..], a)
-        else
-            RestrictTraceToActor(t[1..], a)
-    }
-
-    /////////////////////////////////////////////////
-    // Reduction trees
-    /////////////////////////////////////////////////
-
-    datatype Tree = Inner(reduced_action:Action, children:seq<Tree>) | Leaf(action:Action)
 }
