ironfleet/src/Dafny/Distributed/Concur/ReductionBasic.i.dfy
@@ -1,0 +1,42 @@
+include "Reduction.i.dfy"
+
+module ReductionBasicModule
+{
+    import opened ReductionModule
+
+    lemma lemma_IfEntriesReducibleAndOneIsntRightMoverThenRestAreLeftMovers(entries:seq<Entry>, pivot_index:int, i:int, j:int)
+        requires 0 <= i < j < |entries|;
+        requires 0 <= pivot_index <= |entries|;
+        requires forall k :: 0 <= k < pivot_index ==> EntryIsRightMover(entries[k]);
+        requires forall k :: pivot_index < k < |entries| ==> EntryIsLeftMover(entries[k]);
+        requires !EntryIsRightMover(entries[i]);
+        ensures  EntryIsLeftMover(entries[j]);
+        decreases j;
+    {
+        assert !(i < pivot_index);
+        assert j > pivot_index;
+    }
+
+    lemma lemma_IfEntriesReducibleThenSuffixIs(entries:seq<Entry>, entries':seq<Entry>, pivot_index:int) returns (new_pivot_index:int)
+        requires |entries| > 0;
+        requires entries' == entries[1..];
+        requires 0 <= pivot_index <= |entries|;
+        requires forall i :: 0 <= i < pivot_index ==> EntryIsRightMover(entries[i]);
+        requires forall i :: pivot_index < i < |entries| ==> EntryIsLeftMover(entries[i]);
+        ensures  0 <= new_pivot_index <= |entries'|;
+        ensures  forall i :: 0 <= i < new_pivot_index ==> EntryIsRightMover(entries'[i]);
+        ensures  forall i :: new_pivot_index < i < |entries'| ==> EntryIsLeftMover(entries'[i]);
+    {
+        if |entries'| == 0 {
+            new_pivot_index := 0;
+            return;
+        }
+        
+        if pivot_index == 0 {
+            new_pivot_index := 0;
+        }
+        else {
+            new_pivot_index := pivot_index - 1;
+        }
+    }
+}
