ironfleet/src/Dafny/Distributed/Concur/ReductionMove.i.dfy
@@ -1,68 +1,10 @@
-include "ActorTraces.i.dfy"
+include "Reduction.i.dfy"
 
-module ReductionModule
+module ReductionMoveModule
 {
-    import opened ActorTraces 
+    import opened ReductionModule
 
-    /////////////////////////////////////////////////
-    // Reduction trees
-    /////////////////////////////////////////////////
-
-    datatype Tree = Inner(reduced_entry:Entry, children:seq<Tree>, pivot_index:int) | Leaf(entry:Entry)
-
-    function GetRootEntry(tree:Tree) : Entry
-    {
-        match tree
-            case Inner(reduced_entry, children, pivot_index) => reduced_entry
-            case Leaf(entry) => entry
-    }
-
-    function GetRootEntries(trees:seq<Tree>) : seq<Entry>
-        ensures  var entries := GetRootEntries(trees);
-                     |entries| == |trees|
-                  && forall i {:trigger GetRootEntry(trees[i])}{:trigger GetRootEntries(trees)[i]} ::
-                         0 <= i < |entries| ==> entries[i] == GetRootEntry(trees[i]);
-    {
-        if |trees| == 0 then [] else [GetRootEntry(trees[0])] + GetRootEntries(trees[1..])
-    }
-
-    predicate EntriesReducibleToEntry(entries:seq<Entry>, entry:Entry)
-    {
-        forall db:seq<SystemState> {:trigger SystemNextEntry(db[0], db[|entries|], entry)} ::
-                |db| == |entries|+1
-             && (forall i {:trigger SystemNextEntry(db[i], db[i+1], entries[i])} ::
-                 0 <= i < |entries| ==> SystemNextEntry(db[i], db[i+1], entries[i]))
-                 ==> SystemNextEntry(db[0], db[|entries|], entry)
-    }
-
-    predicate TreeChildrenReducibleToTreeRoot(tree:Tree)
-    {
-        tree.Inner? ==> EntriesReducibleToEntry(GetRootEntries(tree.children), GetRootEntry(tree))
-    }
-
-    predicate TreeRootPivotValid(tree:Tree)
-    {
-        tree.Inner? && |tree.children| > 0 ==>
-               0 <= tree.pivot_index < |tree.children|
-            && (forall i {:trigger EntryIsRightMover(GetRootEntry(tree.children[i]))} ::
-                     0 <= i < tree.pivot_index ==> EntryIsRightMover(GetRootEntry(tree.children[i]))) 
-            && (forall i {:trigger EntryIsLeftMover(GetRootEntry(tree.children[i]))} ::
-                     tree.pivot_index < i < |tree.children| ==> EntryIsRightMover(GetRootEntry(tree.children[i])))
-    }
-
-    predicate TreeRootValid(tree:Tree)
-    {
-           TreeRootPivotValid(tree)
-        && TreeChildrenReducibleToTreeRoot(tree)
-    }
-
-    predicate TreeValid(tree:Tree)
-    {
-           TreeRootValid(tree)
-        && tree.Inner? ==> forall child {:trigger child in tree.children} :: child in tree.children ==> TreeRootValid(child)
-    }
-
-
+/*
     lemma lemma_PerformMoveRight(
         trace:Trace,
         db:seq<SystemState>,
@@ -73,7 +15,7 @@ module ReductionModule
         )
         requires IsValidSystemTraceAndBehavior(trace, db);
         requires 0 <= first_entry_pos < |trace| - 1;
-        requires GetEntryActor(trace[first_entry_pos]) != GetEntryActor(trace[first_entry_pos+1]);
+        requires trace[first_entry_pos].actor != trace[first_entry_pos+1].actor;
         requires EntryIsRightMover(trace[first_entry_pos]);
         ensures  IsValidSystemTraceAndBehavior(trace', db');
         ensures  |db'| == |db|;
@@ -111,7 +53,7 @@ module ReductionModule
         )
         requires IsValidSystemTraceAndBehavior(trace, db);
         requires 0 <= first_entry_pos < |trace| - 1;
-        requires GetEntryActor(trace[first_entry_pos]) != GetEntryActor(trace[first_entry_pos+1]);
+        requires trace[first_entry_pos].actor != trace[first_entry_pos+1].actor;
         requires EntryIsLeftMover(trace[first_entry_pos+1]);
         ensures  IsValidSystemTraceAndBehavior(trace', db');
         ensures  |db'| == |db|;
@@ -478,7 +420,7 @@ module ReductionModule
         requires EntryGroupValid(group);
         requires group == RestrictEntriesToLevel(group, group[0].begin_group_level);
         requires forall i :: begin_entry_pos < i < end_entry_pos ==> trace[i].EntryAction?;
-        requires forall i :: begin_entry_pos <= i <= end_entry_pos ==> GetEntryActor(trace[i]) == actor;
+        requires forall i :: begin_entry_pos <= i <= end_entry_pos ==> trace[i].actor == actor;
         requires forall i :: begin_entry_pos <= i <= end_entry_pos ==> GetEntryLevel(trace[i]) == level;
         requires EntriesReducibleUsingPivot(group);
         requires EntriesReducibleToEntry(group, last(group).reduced_entry);
