ironfleet/src/Dafny/Distributed/Concur/ReductionPreserves.i.dfy
@@ -1,0 +1,477 @@
+include "Reduction.i.dfy"
+
+module ReductionPreservesModule
+{
+    import opened ReductionModule
+
+/*
+    lemma lemma_SeqOffsetSlice<T>(s:seq<T>, offset:int, b1:int, e1:int, b2:int, e2:int)
+        requires 0 <= offset < |s|;
+        requires b2 == b1 - offset;
+        requires e2 == e1 - offset;
+        requires 0 <= b1 < e1 <= |s|;
+        requires 0 <= b2 < e2 <= |s| - offset;
+        ensures  s[b1..e1] == s[offset..][b2..e2];
+    { }
+
+    lemma lemma_SeqOffsetSliceFull<T>(s:seq<T>, b1:int, e1:int, b2:int, e2:int, b3:int, e3:int)
+        requires 0 <= b1 < e1 <= |s|;
+        requires 0 <= b2 < e2 <= |s|;
+        requires 0 <= b3 < e3 <= |s|;
+        requires e3 <= e2 - b2;
+        requires b1 == b3 + b2;
+        requires e1 == b2 + e3;
+        ensures  s[b1..e1] == s[b2..e2][b3..e3];
+    { 
+        var s1 := s[b1..e1];
+        var s2 := s[b2..e2];
+        var s3 := s2[b3..e3];
+        forall i | 0 <= i < |s1| 
+            ensures s1[i] == s3[i];
+        {
+            calc {
+                s1[i];
+                s[b1 + i];
+                s[i+b3+b2];
+                s2[i+b3];
+                s3[i];
+            }
+        }
+    }
+
+    lemma lemma_SeqIndexSliceSlice<T>(s:seq<T>, b1:int, e1:int, b2:int, e2:int, index:int)
+        requires 0 <= b1 <= e1 <= |s|;
+        requires 0 <= b2 <= e2 <= e1 - b1;
+        requires b1 + b2 <= index < b1+e2;
+        ensures  s[index] in s[b1..e1][b2..e2];
+    {
+    }
+
+    lemma lemma_EntryGroupEndsUnique(
+            trace:Trace,
+            min_level:int,
+            max_level:int,
+            start:int,
+            start':int,
+            end:int)
+        requires ActorTraceValid(trace, min_level, max_level);
+        requires 0 <= start < start' < end <= |trace|;
+        requires exists level :: EntryGroupValidForLevels(trace[start ..end], min_level, level); 
+        requires exists level :: EntryGroupValidForLevels(trace[start'..end], min_level, level);
+        requires forall i :: 0 <= i < |trace| ==> GetEntryActor(trace[i]) == GetEntryActor(trace[0]);
+        requires trace[start'].EntryBeginGroup? && trace[start'].begin_group_level == min_level;
+        ensures  false;
+    {
+        calc ==> {
+            trace[start'].begin_group_level == min_level;
+            last(trace[start'..end]).end_group_level == min_level;
+            trace[start].begin_group_level == min_level;
+        }
+        var inner_group := trace[start..end][1..end-start-1];
+        assert trace[start'] in inner_group;
+
+        lemma_IfActorTraceValidWithMinLevelEqualMaxLevelThenAllAreActions(inner_group, min_level);
+    }
+
+//    lemma lemma_ReductionPreservesEntryGroupValidForLevelsHelper(
+//            trace:Trace,
+//            trace':Trace,
+//            level:int,
+//            min_level:int,
+//            mid_level:int,
+//            max_level:int,
+//            position:int,
+//            group_len:int,
+//            i:int
+//            )
+//        requires 0 < position < position + group_len < |trace|;
+//        requires min_level < mid_level <= max_level;
+//        requires EntryGroupValidForLevels(trace, min_level, max_level);
+//        requires EntryGroupValidForLevels(trace[position..position+group_len], min_level, mid_level);
+//        requires level == trace[0].begin_group_level;
+//        requires mid_level <= trace[0].begin_group_level;
+//        requires trace[position].EntryBeginGroup? && trace[position].begin_group_level == min_level;
+//        requires forall j :: 0 <= j < |trace| ==> GetEntryActor(trace[j]) == GetEntryActor(trace[0]);
+//        requires trace' == trace[..position] + [trace[position+group_len-1].reduced_entry] + trace[position + group_len..];
+//        requires ActorTraceValid(middle(trace'), min_level, trace'[0].begin_group_level);
+//        requires 0 <= i < |RestrictEntriesToLevel(trace, level)|;
+//        ensures  i <= |RestrictEntriesToLevel(trace', level)|;
+//        ensures  |RestrictEntriesToLevel(trace, level)[i..]| == |RestrictEntriesToLevel(trace', level)[i..]|;
+//        ensures  forall j :: i <= j < |RestrictEntriesToLevel(trace, level)| ==>
+//                 RestrictEntriesToLevel(trace, level)[j] == RestrictEntriesToLevel(trace', level)[j];
+//    {
+//        var restricted_trace  := RestrictEntriesToLevel(trace,  level);
+//        var restricted_trace' := RestrictEntriesToLevel(trace', level);
+//
+////        if 
+////
+////        if trace == [] then []
+////        else if GetEntryLevel(trace[0]) == level then
+////            [trace[0]] + RestrictEntriesToLevel(trace[1..], level)
+////        else if trace[0].EntryEndGroup? && GetEntryLevel(trace[0].reduced_entry) == level then
+////            [trace[0].reduced_entry] + RestrictEntriesToLevel(trace[1..], level)
+////        else 
+////            RestrictEntriesToLevel(trace[1..], level)
+//    }
+
+    lemma lemma_ReductionPreservesEntryGroupValidForLevels(
+            trace:Trace,
+            trace':Trace,
+            min_level:int,
+            mid_level:int,
+            max_level:int,
+            position:int,
+            group_len:int
+            )
+        requires 0 < position < position + group_len < |trace|;
+        requires min_level < mid_level <= max_level;
+        requires EntryGroupValidForLevels(trace, min_level, max_level);
+        requires EntryGroupValidForLevels(trace[position..position+group_len], min_level, mid_level);
+        requires mid_level <= trace[0].begin_group_level;
+        requires trace[position].EntryBeginGroup? && trace[position].begin_group_level == min_level;
+        requires forall i :: 0 <= i < |trace| ==> GetEntryActor(trace[i]) == GetEntryActor(trace[0]);
+        requires trace' == trace[..position] + [trace[position+group_len-1].reduced_entry] + trace[position + group_len..];
+        requires ActorTraceValid(middle(trace'), min_level, trace'[0].begin_group_level);
+        ensures  EntryGroupValidForLevels(trace', min_level, max_level);
+    {
+        assert trace[0] == trace'[0];
+        var level := trace[0].begin_group_level;
+        var restricted_trace  := RestrictEntriesToLevel(trace,  level);
+        var restricted_trace' := RestrictEntriesToLevel(trace', level);
+
+        reveal_RestrictEntriesToLevel();
+
+        calc {
+            RestrictEntriesToLevel(trace, level);
+                { lemma_RestrictEntriesToLevelAdds(trace[..position], trace[position..], level); 
+                  assert trace == trace[..position] + trace[position..]; }
+            RestrictEntriesToLevel(trace[..position], level) + RestrictEntriesToLevel(trace[position..], level);
+                { lemma_RestrictEntriesToLevelAdds(trace[position..position+group_len], trace[position+group_len..], level); 
+                  assert trace[position..] == trace[position..position+group_len] + trace[position+group_len..]; } 
+            RestrictEntriesToLevel(trace[..position], level) + RestrictEntriesToLevel(trace[position..position+group_len], level) + RestrictEntriesToLevel(trace[position+group_len..], level);
+
+            RestrictEntriesToLevel(trace[..position], level) + RestrictEntriesToLevel([trace[position+group_len-1].reduced_entry], level) + RestrictEntriesToLevel(trace[position+group_len..], level);
+                { lemma_RestrictEntriesToLevelAdds([trace[position+group_len-1].reduced_entry], trace[position+group_len..], level); } 
+            RestrictEntriesToLevel(trace[..position], level) + RestrictEntriesToLevel(trace'[position..], level);
+                { assert trace'[..position] == trace[..position]; }
+            RestrictEntriesToLevel(trace'[..position], level) + RestrictEntriesToLevel(trace'[position..], level);
+                { lemma_RestrictEntriesToLevelAdds(trace'[..position], trace'[position..], level); 
+                  assert trace' == trace'[..position] + trace'[position..]; }
+            RestrictEntriesToLevel(trace', level);
+        }
+
+//        lemma_ReductionPreservesEntryGroupValidForLevelsHelper(trace, trace', level, min_level, mid_level, max_level, position, group_len, 0);
+//        assert restricted_trace == restricted_trace';
+//
+////        forall i :: 0 <= i < |restricted_trace|
+////            ensures restricted_trace[i] == restricted_trace'[i];
+////        {
+////            assert restricted_trace[i] in restricted_trace;
+////            lemma_RestrictEntriesToLevelProperties(trace, level);
+////            var j :| EntryCorrespondsToEntryWhenRestrictedToLevel(restricted_trace[i], trace, j, level);
+////            if j < position
+////        }
+////
+////        assert |restricted_trace| == |restricted_trace'|;
+    }
+
+    lemma {:timeLimitMultiplier 4} lemma_ReductionPreservesActorTraceValidProperSubset(
+            trace:Trace,
+            min_level:int,
+            mid_level:int,
+            max_level:int,
+            position:int,
+            group_len:int,
+            g_len:int,
+            trace':Trace)
+        requires ActorTraceValid(trace, min_level, max_level);
+        requires 0 < position < position + group_len <= |trace|;
+        requires min_level < mid_level <= max_level;
+        requires EntryGroupValidForLevels(trace[position..position+group_len], min_level, mid_level);
+        requires 0 < g_len <= |trace| && EntryGroupValidForLevels(trace[..g_len], min_level, max_level)
+              && ActorTraceValid(trace[g_len..], min_level, max_level);
+        requires position + group_len < g_len;
+        requires mid_level <= trace[0].begin_group_level;
+        requires trace[position].EntryBeginGroup? && trace[position].begin_group_level == min_level;
+        requires forall i :: 0 <= i < |trace| ==> GetEntryActor(trace[i]) == GetEntryActor(trace[0]);
+        requires trace' == trace[..position] + [trace[position+group_len-1].reduced_entry] + trace[position + group_len..];
+        decreases |trace|, 0;
+        ensures  ActorTraceValid(trace', min_level, max_level);
+    {
+        var sub_trace := trace[..g_len];
+        var mid_sub_trace := sub_trace[1..g_len-1];
+        assert ActorTraceValid(mid_sub_trace, min_level, sub_trace[0].begin_group_level);
+
+        calc {
+            mid_sub_trace[position-1..position-1+group_len];
+                { lemma_SeqOffsetSliceFull(sub_trace, position, position+group_len, 1, g_len-1, position-1, position-1+group_len); }
+            sub_trace[position..position+group_len];
+            trace[position..position+group_len];
+        }
+
+        var new_trace' := mid_sub_trace[..position-1] + [mid_sub_trace[position+group_len-2].reduced_entry] + mid_sub_trace[position-1 + group_len..];
+        lemma_ReductionPreservesActorTraceValid(mid_sub_trace, min_level, mid_level, trace[0].begin_group_level, position-1, group_len, new_trace');
+
+        calc {
+            |trace'|;
+            position + 1 + |trace| - (position + group_len);
+            1 + |trace| - group_len;
+            1 + g_len - 1 - group_len + 1 + |trace| - g_len;
+            calc {
+                g_len - 1 - group_len;
+                position - 1 + 1 + (g_len-1-1) - (position-1+group_len);
+                position - 1 + 1 + |mid_sub_trace| - (position-1+group_len);
+                |mid_sub_trace[..position-1] + [mid_sub_trace[position+group_len-2].reduced_entry] + mid_sub_trace[position-1 + group_len..]|;
+                |new_trace'|;
+            }
+            1 + |new_trace'| + 1 + |trace| - g_len;
+            1 + |new_trace'| + 1 + |trace| - g_len;
+            |[trace[0]] + new_trace' + [trace[g_len-1]] + trace[g_len..]|;
+        }
+        calc {
+            trace';
+            [trace[0]] + new_trace' + [trace[g_len-1]] + trace[g_len..];
+        //   Begin    ActorTraceValid    End             ActorTraceValid
+        }
+        assert trace[..g_len][position..position+group_len] == trace[position..position+group_len];
+        assert trace'[..g_len-group_len+1] == trace[..position] + [trace[position+group_len-1].reduced_entry] + trace[position + group_len..g_len];
+        lemma_ReductionPreservesEntryGroupValidForLevels(trace[..g_len], trace'[..g_len - group_len + 1], 
+            min_level, mid_level, max_level, position, group_len);
+        assert EntryGroupValidForLevels(trace'[..g_len - group_len + 1], min_level, max_level);
+
+    }
+
+    lemma lemma_ReductionPreservesActorTraceValid(
+            trace:Trace,
+            min_level:int,
+            mid_level:int,
+            max_level:int,
+            position:int,
+            group_len:int,
+            trace':Trace)
+        requires ActorTraceValid(trace, min_level, max_level);
+        requires 0 <= position < position + group_len <= |trace|;
+        requires min_level < mid_level <= max_level;
+        requires EntryGroupValidForLevels(trace[position..position+group_len], min_level, mid_level);
+        requires trace[position].EntryBeginGroup? && trace[position].begin_group_level == min_level;
+        requires forall i :: 0 <= i < |trace| ==> GetEntryActor(trace[i]) == GetEntryActor(trace[0]);
+        requires trace' == trace[..position] + [trace[position+group_len-1].reduced_entry] + trace[position + group_len..];
+        decreases |trace|, 1;
+        ensures  ActorTraceValid(trace', min_level, max_level);
+/*
+    {
+        if position == 0 {
+            var g_len :|    0 < g_len <= |trace|
+                      && EntryGroupValidForLevels(trace[..g_len], min_level, max_level)
+                      && ActorTraceValid(trace[g_len..], min_level, max_level);
+            var entry_group := trace[position..position+group_len];
+            if g_len < group_len {
+                var inner_group := entry_group[1..|entry_group|-1];
+                lemma_SeqIndexSliceSlice(trace, position, position+group_len, 1, |entry_group|-1, g_len-1);
+                assert trace[g_len - 1] in inner_group;
+                lemma_IfActorTraceValidWithMinLevelEqualMaxLevelThenAllAreActions(inner_group, min_level);
+                assert false;
+            } else if g_len > group_len {
+                var inner_group := trace[..g_len][1..g_len-1];
+                lemma_SeqIndexSliceSlice(trace, 0, g_len, 1, g_len-1, group_len-1);
+                assert trace[group_len-1] in inner_group;
+                lemma_IfActorTraceValidWithMinLevelEqualMaxLevelThenAllAreActions(inner_group, min_level);
+                assert false;
+            }
+            assert ActorTraceValid(trace', min_level, max_level);
+        } else {
+            if trace[0].EntryAction? && GetEntryLevel(trace[0]) == max_level && ActorTraceValid(trace[1..], min_level, max_level) {
+                lemma_SeqOffsetSlice(trace, 1, position, position+group_len, position-1, position+group_len-1);
+                assert trace[1..][position-1..position-1+group_len] == trace[position..position+group_len];
+                lemma_ReductionPreservesActorTraceValid(trace[1..], min_level, mid_level, max_level, position-1, group_len, trace'[1..]);
+                assert ActorTraceValid(trace', min_level, max_level);
+            } else {
+                assert exists g_len ::    0 < g_len <= |trace|
+                          && EntryGroupValidForLevels(trace[..g_len], min_level, max_level)
+                          && ActorTraceValid(trace[g_len..], min_level, max_level);
+                var g_len :|    0 < g_len <= |trace|
+                          && EntryGroupValidForLevels(trace[..g_len], min_level, max_level)
+                          && ActorTraceValid(trace[g_len..], min_level, max_level);
+
+                if position < g_len {
+                    if !(position + group_len < g_len) {
+                        var end := last(trace[..g_len]);
+                        assert end.EntryEndGroup?;
+
+                        var entry_group := trace[position..position + group_len];
+
+                        if position + group_len == g_len {
+                            assert end == last(entry_group);
+                            assert EntryGroupValidForLevels(trace[0..position+group_len], min_level, max_level);
+                            lemma_EntryGroupEndsUnique(trace, min_level, max_level, 0, position, position+group_len);
+                            assert false;
+                        }
+
+
+                        var inner_group := entry_group[1..|entry_group|-1];
+                        if end in inner_group {
+                            lemma_IfActorTraceValidWithMinLevelEqualMaxLevelThenAllAreActions(inner_group, min_level);
+                            assert end.EntryAction?;
+                            assert false;
+                        } else {
+                            assert end in entry_group;
+                            var end_index :| 0 <= end_index < |entry_group| && entry_group[end_index] == end;
+                            if 0 < end_index < |entry_group| - 1 {
+                                assert end in inner_group;
+                                assert false;
+                            } else if end_index == 0 {
+                                assert end != entry_group[0];
+                                assert false;
+                            } else {
+                                calc {
+                                    end_index;
+                                    |entry_group| - 1;
+                                    group_len - 1;
+                                }
+                                assert entry_group[group_len-1] == trace[position + group_len - 1];
+                                assert position + group_len - 1 != g_len - 1;
+                                assert trace[position+group_len-1] == trace[g_len-1];
+                                assert trace[0].EntryBeginGroup? && trace[0].begin_group_level == min_level;
+                                var inner_group' := trace[..g_len][1..g_len-1];
+                                lemma_IfActorTraceValidWithMinLevelEqualMaxLevelThenAllAreActions(inner_group', min_level);
+                                lemma_SeqIndexSliceSlice(trace, 0, g_len, 1, g_len-1, position);
+                                assert trace[position] in inner_group';
+                                assert false;
+                            }
+                        }
+                    } else {
+                        lemma_ReductionPreservesActorTraceValidProperSubset(trace, min_level, mid_level, max_level, position, group_len, g_len, trace');
+                    }
+                    assert ActorTraceValid(trace', min_level, max_level);
+                } else {
+                    lemma_SeqOffsetSlice(trace, g_len, position, position+group_len,
+                                         position-g_len, position-g_len+group_len);
+                    assert trace[g_len..][position-g_len..position-g_len+group_len] == trace[position..position+group_len];
+                    calc {
+                        trace'[g_len..];
+                        (trace[..position] + [trace[position+group_len-1].reduced_entry] + trace[position + group_len..])[g_len..]; 
+                            { assert |trace[..position]| >= g_len; }
+                        trace[..position][g_len..] + [trace[position+group_len-1].reduced_entry] + trace[position + group_len..]; 
+                        trace[g_len..position] + [trace[position+group_len-1].reduced_entry] + trace[position + group_len..]; 
+                            { assert trace[g_len..position] == trace[g_len..][..position-g_len]; }
+                        trace[g_len..][..position-g_len] + [trace[position+group_len-1].reduced_entry] + trace[position + group_len..]; 
+                            { assert trace[position+group_len-1] == trace[g_len..][position-g_len+group_len-1]; }
+                        trace[g_len..][..position-g_len] + [trace[g_len..][position-g_len+group_len-1].reduced_entry] + trace[position + group_len..]; 
+                            { assert trace[position + group_len..] == trace[g_len..][position-g_len + group_len..]; }
+                        trace[g_len..][..position-g_len] + [trace[g_len..][position-g_len+group_len-1].reduced_entry] + trace[g_len..][position-g_len + group_len..]; 
+                    }
+                    lemma_ReductionPreservesActorTraceValid(trace[g_len..], min_level, mid_level, max_level, position-g_len, group_len, trace'[g_len..]);
+                    assert ActorTraceValid(trace[g_len..], min_level, max_level);
+                    assert ActorTraceValid(trace'[g_len..], min_level, max_level);
+                    assert trace'[..g_len] == trace[..g_len];
+                    assert    0 < g_len <= |trace'|
+                              && EntryGroupValidForLevels(trace'[..g_len], min_level, max_level)
+                              && ActorTraceValid(trace'[g_len..], min_level, max_level);
+                    assert ActorTraceValid(trace', min_level, max_level);
+                }
+            }
+        }
+    }
+*/
+    lemma lemma_ReductionPreservesTraceValid(
+            trace:Trace,
+            min_level:int,
+            mid_level:int,
+            max_level:int,
+            position:int,
+            group_len:int)
+        returns (trace':Trace)
+        requires TraceValid(trace, min_level, max_level);
+        requires min_level < mid_level <= max_level;
+        requires 0 <= position < position + group_len <= |trace|;
+        requires EntryGroupValidForLevels(trace[position..position+group_len], min_level, mid_level);
+        requires trace[position].EntryBeginGroup? && trace[position].begin_group_level == min_level;
+        requires forall i :: position <= i < position+group_len ==> GetEntryActor(trace[i]) == GetEntryActor(trace[position]);
+        ensures  trace' == trace[..position] + [trace[position+group_len-1].reduced_entry] + trace[position + group_len..];
+        ensures  TraceValid(trace', min_level, max_level);
+    {
+
+        trace' := trace[..position] + [trace[position+group_len-1].reduced_entry] + trace[position + group_len..];
+        var this_actor := GetEntryActor(trace[position]);
+        forall actor
+            ensures ActorTraceValid(RestrictTraceToActor(trace', actor), min_level, max_level);
+        {
+            if actor == this_actor {
+                var _, actor_trace, actor_indices, actor_indices_index := GetCorrespondingActorTraceAndIndexForEntry(trace, position);
+                var a_trace := RestrictTraceToActor(trace', actor);
+
+                forall i | 0 <= i < group_len
+                    ensures 0 <= actor_indices_index + i < |actor_trace|;
+                    ensures actor_indices[actor_indices_index+i] == position+i;
+                    ensures actor_trace[actor_indices_index+i] == trace[position+i];
+                {  
+                    lemma_TraceIndicesForActor_length(trace, actor);
+                    lemma_ConsecutiveActorEntries(trace, position, group_len, actor_indices_index, i);
+                }
+
+                var j := group_len-1;
+                assert 0 <= actor_indices_index+j < |actor_trace|;
+                assert 0 <= actor_indices_index+(group_len-1) < |actor_trace|;
+
+                var actor_trace_subset := actor_trace[actor_indices_index..actor_indices_index+group_len];
+                var trace_subset := trace[position..position+group_len];
+                assert |actor_trace_subset| == |trace_subset|;
+                forall i | 0 <= i < |actor_trace_subset| 
+                    ensures actor_trace_subset[i] == trace_subset[i];
+                {
+                    calc {
+                        actor_trace_subset[i];
+                            { lemma_ElementFromSequenceSlice(actor_trace, actor_trace_subset, 
+                                                             actor_indices_index, actor_indices_index+group_len, actor_indices_index+i); }
+                        actor_trace[actor_indices_index+i];
+                        trace[position + i];
+                            { lemma_ElementFromSequenceSlice(trace, trace_subset, 
+                                                             position, position+group_len, position+i); }
+                        trace_subset[i];
+                    }
+                }                
+                assert actor_trace_subset == trace_subset;
+                assert actor_trace[actor_indices_index+j] == trace[position + j];
+                assert actor_trace[actor_indices_index+j].EntryEndGroup?;
+                assert actor_trace[actor_indices_index+group_len-1] == actor_trace[actor_indices_index+j];
+
+                var b_trace := actor_trace[..actor_indices_index] + [actor_trace[actor_indices_index+group_len-1].reduced_entry] + actor_trace[actor_indices_index + group_len..];
+
+                calc {
+                    a_trace;
+                    RestrictTraceToActor(trace', actor);
+                    RestrictTraceToActor(trace[..position] + [trace[position+group_len-1].reduced_entry] + trace[position + group_len..], actor);
+                        { lemma_SplitRestrictTraceToActor(trace[..position] + [trace[position+group_len-1].reduced_entry], trace[position + group_len..], actor); }
+                    RestrictTraceToActor(trace[..position] + [trace[position+group_len-1].reduced_entry], actor) + RestrictTraceToActor(trace[position + group_len..], actor);
+                        { lemma_SplitRestrictTraceToActor(trace[..position], [trace[position+group_len-1].reduced_entry], actor); }
+                    RestrictTraceToActor(trace[..position], actor) + RestrictTraceToActor([trace[position+group_len-1].reduced_entry], actor) + RestrictTraceToActor(trace[position + group_len..], actor);
+                        { lemma_RestrictTraceToActorSeqSliceTake(trace, actor, position, actor_indices_index); }
+                    actor_trace[..actor_indices_index] + RestrictTraceToActor([trace[position+group_len-1].reduced_entry], actor) + RestrictTraceToActor(trace[position + group_len..], actor);
+                        { lemma_RestrictTraceToActorSeqSliceDrop(trace, actor, position+j, actor_indices_index+j); 
+                          assert position + j + 1 == position + group_len;
+                          assert actor_indices_index+j+1 == actor_indices_index+group_len;
+                        }
+                    actor_trace[..actor_indices_index] + RestrictTraceToActor([trace[position+group_len-1].reduced_entry], actor) + actor_trace[actor_indices_index + group_len..];
+                        { assert position+group_len-1 == position + j;
+                          assert trace[position+group_len-1] == trace[position + j]; 
+                          assert position <= position + j < position + group_len;
+                        }
+                    actor_trace[..actor_indices_index] + [actor_trace[actor_indices_index+group_len-1].reduced_entry] + actor_trace[actor_indices_index + group_len..];
+                    b_trace;
+
+                }
+
+                assert a_trace == b_trace;
+
+                lemma_ReductionPreservesActorTraceValid(actor_trace, min_level, mid_level, max_level, actor_indices_index, group_len, a_trace);
+                assert ActorTraceValid(RestrictTraceToActor(trace', actor), min_level, max_level);
+            } else {
+                lemma_RestrictTraceToActorPreservation(trace, this_actor, position, position+group_len-1,
+                                                       trace[position+group_len-1].reduced_entry, trace');
+                assert ActorTraceValid(RestrictTraceToActor(trace', actor), min_level, max_level);
+            }
+        }
+    }
+*/
+
+}
